\documentclass[12pt]{report}
\usepackage{amsmath,amssymb}
\usepackage[margin=2.4 cm]{geometry}
\usepackage{graphicx}
\usepackage{color}
\graphicspath{{images/}}
\usepackage{float}
\usepackage{sidecap}
\usepackage{subcaption}
\usepackage{braket}
\usepackage{pdfpages}
\usepackage{rotating}
\usepackage{lineno}
\usepackage{array}
\usepackage{cite}
\usepackage[utf8]{inputenc}
\usepackage[bottom]{footmisc}
\usepackage[toc,page]{appendix}
\usepackage{amssymb}




\sidecaptionvpos{figure}{c}
\linespread{1.3}
\begin{document}
\begin{equation}
f_i(H_i|\theta)=\frac{M_i(\theta)^{H_i}}{H_i!}e^{-M_i(\theta)}/\frac{M_i(\hat{\theta})^{H_i}}{H_i!}e^{-M_i(\hat{\theta})}=\left(\frac{M_i(\theta)}{M_i(\hat{\theta})}\right)^{H_i}e^{-(M_i(\theta)-M_i(\hat{\theta}))}
\end{equation}
\begin{equation}
F(H|\theta)=\prod_if_i
\end{equation}
\begin{equation}
L(H|\theta)=-\text{Log}(F(H|\theta))=-\sum_il_i(H_i|\theta)
\end{equation}
\begin{equation}
l_i(H_i|\theta)=\text{Log}(f_i(H_i|\theta))=H_i\left[\text{Log}(M_i(\theta))-\text{Log}(M_i(\hat{\theta}))\right]-M_i(\theta)+M_i(\hat{\theta})
\end{equation}
Fisher Information:
\begin{equation}
I=E\left[(\partial_\theta L(H|\theta))^2_{\theta_0}\right]=\sum_iE\left[(\partial_\theta l_i(H_i|\theta))^2_{\theta_0}\right]
\end{equation}
\begin{equation}
\partial_\theta l_i(H_i|\theta_0)=\frac{\partial_\theta f_i(H_i|\theta_0)}{f_i(H_i|\theta_0)}
\end{equation}
\begin{equation}
\partial_\theta f_i(H_i|\theta_0)=\left(\frac{M'_i(\theta_0)}{M_i(\theta_0)}H_i-M'_i(\theta_0)\right)f_i(H_i|\theta)
\end{equation}
\begin{equation}
\begin{split}
I&=\sum_i(M'_i(\theta_0))^2E\left[\frac{H_i^2}{M_i^2(\theta_0)}-2\frac{H_i}{M_i(\theta_0)}+1\right]=\sum_i(M'_i(\theta_0))^2\left(\frac{E[H_i^2]}{M_i^2(\theta_0)}-2\frac{E[H_i]}{M_i(\theta_0)}+1\right)\\
&=\sum_i(M'_i(\theta_0))^2\left(\frac{Var[H_i]+E^2[H_i]}{M_i^2(\theta_0)}-2\frac{E[H_i]}{M_i(\theta_0)}+1\right)=\sum_i\frac{(M_i'(\theta_0))^2}{M_i(\theta_0)}
\end{split}
\end{equation}
****
\begin{equation}
E[\partial^2_\theta L(H|\theta)]=\sum_iE\left[\frac{\partial^2_\theta f_i(H_i|\theta_0)}{f_i(H_i|\theta_0)}-\frac{(\partial_{\theta}f_i(H_i|\theta_0))^2}{f_i^2(H_i|\theta_0)}\right]=\sum_iE\left[\frac{\partial^2_\theta f_i(H_i|\theta_0)}{f_i(H_i|\theta_0)}\right]-I=-I
\end{equation}
\begin{equation}
\partial^2_\theta f_i(H_i|\theta_0)=f_i(H_i|\theta_0)\left(\frac{M_i''}{M_i}H_i-\frac{(M'_i)^2}{M_i^2}H_i-M''_i+\frac{(M'_i)^2}{M_i^2}H_i^2-2\frac{(M'_i)^2}{M_i}H_i+(M'_i)^2\right)
\end{equation}
\begin{equation}
\sum_iE\left[\frac{\partial^2_\theta f_i(H_i|\theta_0)}{f_i(H_i|\theta_0)}\right]=\left(M_i''-\frac{(M'_i)^2}{M_i}-M''_i+\frac{(M'_i)^2}{M_i}+(M'_i)^2-2(M'_i)^2+(M'_i)^2\right)=0
\end{equation}
We want to evaluate $L(H|\theta)$ near $\hat{\theta}$,
\begin{equation}
\begin{split}
L(H|\Delta\theta)=&-\sum_iH_i\text{Log}\left(1+\frac{M'_i(\hat{\theta})}{M_i(\hat\theta)}\Delta\theta\right)-M'_i(\hat{\theta})\Delta\theta=\\
&-\sum_iH_i\left(\frac{M'_i(\hat{\theta})}{M_i(\hat{\theta})}\Delta\theta-\frac{1}{2}\left(\frac{M'_i(\hat{\theta})}{M_i(\hat{\theta})}\right)^2\Delta\theta^2\right)-M'_i(\hat{\theta})\Delta\theta=\\
&\frac{\Delta\theta^2}{2}\sum_i\left(\frac{M'_i(\hat{\theta})}{M_i(\hat{\theta})}\right)^2H_i+\Delta\theta\partial_\theta F(H|\hat{\theta})=\frac{\Delta\theta^2}{2}\sum_i\left(\frac{M'_i(\hat{\theta})}{M_i(\hat{\theta})}\right)^2H_i
\end{split}
\end{equation}
******
\begin{equation}
0=L'(H|\hat{\theta})=L'(H|\theta_0)+L''(H|\theta_0)\Delta\theta_0 \rightarrow \Delta\theta_0=-\frac{L'(H|\theta_0)}{L''(H|\theta_0)}=-\frac{\sum_il_i'(H_i|\theta_0)}{\sum_il_i''(H_i|\theta_0)}
\end{equation}
\begin{equation}
0=E[L'(H|\theta_0)] \quad E[L''(H|\theta_0)]=-I
\end{equation}
\begin{equation}
\Delta\theta_0=-\frac{\sqrt{n}(1/n\sum_il'_i-E[L'])}{\sqrt{n}(1/n\sum_il''_i-E[L''])-\sqrt{n}I}
\end{equation}
\begin{equation}
\sqrt{n}I\Delta\theta_0\sim\text{Norm}(0,Var[L']) \rightarrow\Delta\theta_0\sim\text{Norm}(0,Var[L']/nI^2)
\end{equation}
\begin{equation}
Var[L']=Var[\sum_i\frac{M_i'}{M_i}H_i-M_i']=\sum_iVar[\frac{M_i'}{M_i}H_i-M_i']=\sum_i\left(\frac{M'_i}{M_i}\right)^2Var[H_i]=I
\end{equation}
\begin{equation}
\Delta\theta_0\sim\text{Norm(0,1/nI)}
\end{equation}
\bibliographystyle{unsrt}
\bibliography{bib} 

\end{document}
